coq/Compiler/Optimizer/TOptimEnvFunc.v
@@ -1759,66 +1759,9 @@ Section TOptimEnvFunc.
   Qed.
   Hint Rewrite @tmerge_empty_record_r_fun_correctness : optim_correct.
 
-  Fixpoint nodupA_checker {fruntime:foreign_runtime} (p:algenv) : bool
-    := match p with
-       | ANUnop ADistinct _ => true
-       | ANBinop AMinus p₁ p₂ => nodupA_checker p₂
-       | _ => false
-       end.
-
-  Lemma nodupA_checker_correct {m:basic_model} (p:algenv) :
-    nodupA_checker p = true -> nodupA p.
-  Proof.
-    induction p; simpl; try discriminate.
-    - destruct b; try discriminate.
-      intros nd.
-      repeat red; intros.
-      destruct d; trivial.
-      simpl in H.
-      unfold olift2 in H.
-      match_case_in H
-      ; intros; rewrite H0 in H; try discriminate.
-      match_case_in H
-      ; intros; rewrite H1 in H; try discriminate.
-      unfold rondcoll2 in H.
-      apply some_lift in H.
-      destruct H as [? ? ?].
-      invcs e0.
-      unfold ondcoll2 in e.
-      match_destr_in e.
-      match_destr_in e.
-      invcs e.
-      apply bminus_NoDup.
-      specialize (IHp2 nd).
-      specialize (IHp2 h c dn_c env dn_env x dn_x _ H1).
-      simpl in IHp2.
-      trivial.
-    - destruct u; try discriminate.
-      intros _ .
-      repeat red; intros.
-      destruct d; trivial.
-      simpl in H.
-      unfold olift in H.
-      match_case_in H
-      ; intros; rewrite H0 in H; try discriminate.
-      unfold rondcoll in H.
-      apply some_lift in H.
-      destruct H as [? ? ?].
-      invcs e0.
-      unfold ondcoll in e.
-      match_destr_in e.
-      invcs e.
-      apply bdistinct_NoDup.
-  Qed.
-    
-  (* optimization for distinct *)
   Definition tdup_elim_fun {fruntime:foreign_runtime} (p:algenv) :=
-    match p with
-    | ANUnop ADistinct q  =>
-      if nodupA_checker q then q else p
-    | _ => p
-    end.
-  
+    dup_elim_fun p.
+
   Lemma tdup_elim_fun_correctness {model:basic_model} (p:algenv) :
     p ⇒ tdup_elim_fun p.
   Proof.
